wip: cleanup

src/SlabsCommon.fst
@@ -294,3 +294,17 @@ let pack_md_array (#opened:_)
   = change_equal_slprop
       (A.varray (A.split_l (A.split_r md_region (u32_to_sz md_count)) (u32_to_sz 1ul)))
       (A.varray (md_array md_region md_count))
+
+let unpack_md_array (#opened:_)
+  (md_region: array AL.cell{A.length md_region = U32.v metadata_max})
+  (md_count: U32.t{U32.v md_count < U32.v metadata_max})
+  : SteelGhost unit opened
+    (A.varray (md_array md_region md_count))
+    (fun _ -> A.varray (A.split_l (A.split_r md_region (u32_to_sz md_count)) 1sz))
+    (requires fun _ -> True)
+    (ensures fun h0 _ h1 ->
+      A.asel (A.split_l (A.split_r md_region (u32_to_sz md_count)) 1sz) h1 ==
+      A.asel (md_array md_region md_count) h0)
+  = change_equal_slprop
+      (A.varray (md_array md_region md_count))
+      (A.varray (A.split_l (A.split_r md_region (u32_to_sz md_count)) 1sz))
